theories/Symbolic/PartialEvaluation.v
@@ -28,6 +28,9 @@
 (******************************************************************************)
 
 From Coq Require Import
+     Arith.PeanoNat
+     Bool.Bool
+     NArith.BinNat
      ZArith.BinInt.
 From Equations Require Import
      Equations.
@@ -117,23 +120,39 @@ Module Type PartialEvaluationOn
     | term_val _ v := term_val (ty.sum _ _) (@inr (Val _) (Val _) v);
     | t            := term_inr t.
 
+    Definition peval_sext {m n} {p : IsTrue (m <=? n)} (t : Term Σ (ty.bvec m)) : Term Σ (ty.bvec n) :=
+      match term_get_val t with
+      | Some v => term_val (ty.bvec n) (bv.sext v)
+      | None   => term_sext t
+      end.
+
+    Definition peval_zext {m n} {p : IsTrue (m <=? n)} (t : Term Σ (ty.bvec m)) : Term Σ (ty.bvec n) :=
+      match term_get_val t with
+      | Some v => term_val (ty.bvec n) (bv.zext v)
+      | None   => term_zext t
+      end.
+
     Definition peval_union {U K} (t : Term Σ (unionk_ty U K)) : Term Σ (ty.union U) :=
       match term_get_val t with
       | Some v => term_val (ty.union U) (unionv_fold U (existT K v))
       | None   => term_union U K t
       end.
 
-    Equations(noeqns) peval [σ] (t : Term Σ σ) : Term Σ σ :=
-    | term_var ς          => term_var ς
-    | term_val _ v        => term_val _ v
-    | term_binop op t1 t2 => peval_binop op (peval t1) (peval t2)
-    | term_neg t          => peval_neg (peval t)
-    | term_not t          => peval_not (peval t)
-    | term_inl t          => peval_inl (peval t)
-    | term_inr t          => peval_inr (peval t)
-    | @term_tuple _ σs ts => @term_tuple _ σs (env.map (fun b => @peval b) ts)
-    | term_union U K t    => peval_union (peval t)
-    | @term_record _ R ts => term_record R (env.map (fun b => peval (σ := type b)) ts).
+    Fixpoint peval [σ] (t : Term Σ σ) : Term Σ σ :=
+      match t with
+      | term_var ς          => term_var ς
+      | term_val _ v        => term_val _ v
+      | term_binop op t1 t2 => peval_binop op (peval t1) (peval t2)
+      | term_neg t          => peval_neg (peval t)
+      | term_not t          => peval_not (peval t)
+      | term_inl t          => peval_inl (peval t)
+      | term_inr t          => peval_inr (peval t)
+      | term_sext t         => peval_sext (peval t)
+      | term_zext t         => peval_zext (peval t)
+      | @term_tuple _ σs ts => @term_tuple _ σs (env.map (fun b => @peval b) ts)
+      | term_union U K t    => peval_union (peval t)
+      | @term_record _ R ts => term_record R (env.map (fun b => peval (σ := type b)) ts)
+      end.
 
     Lemma peval_neg_sound (t : Term Σ ty.int) :
       forall (ι : Valuation Σ),
@@ -159,6 +178,22 @@ Module Type PartialEvaluationOn
         inst (peval_inr (σ1 := σ1) t) ι = inst (term_inr t) ι.
     Proof. destruct t; cbn; auto. Qed.
 
+    Lemma peval_sext_sound {m n} {p : IsTrue (m <=? n)} (t : Term Σ (ty.bvec m)) :
+      forall (ι : Valuation Σ),
+        inst (peval_sext t) ι = inst (term_sext t) ι.
+    Proof.
+      intros ι. unfold peval_sext.
+      destruct (term_get_val_spec t); cbn; subst; easy.
+    Qed.
+
+    Lemma peval_zext_sound {m n} {p : IsTrue (m <=? n)} (t : Term Σ (ty.bvec m)) :
+      forall (ι : Valuation Σ),
+        inst (peval_zext t) ι = inst (term_zext t) ι.
+    Proof.
+      intros ι. unfold peval_zext.
+      destruct (term_get_val_spec t); cbn; subst; easy.
+    Qed.
+
     Lemma peval_union_sound {U K} (t : Term Σ (unionk_ty U K)) :
       forall (ι : Valuation Σ),
         inst (peval_union t) ι = inst (term_union U K t) ι.
@@ -181,6 +216,8 @@ Module Type PartialEvaluationOn
       - now rewrite peval_not_sound, IHt.
       - now rewrite peval_inl_sound, IHt.
       - now rewrite peval_inr_sound, IHt.
+      - now rewrite peval_sext_sound, IHt.
+      - now rewrite peval_zext_sound, IHt.
       - f_equal. induction IH; cbn; f_equal; auto.
       - now rewrite peval_union_sound, IHt.
       - f_equal. induction IH; cbn; f_equal; auto.
