theories/Symbolic/Propositions.v
@@ -27,6 +27,8 @@
 (******************************************************************************)
 
 From Coq Require Import
+     Arith.PeanoNat
+     Bool.Bool
      Classes.Morphisms
      Classes.RelationClasses
      Lists.List
@@ -1444,6 +1446,8 @@ Module Type SymPropOn
     | eterm_not     (t : ETerm ty.bool) : ETerm ty.bool
     | eterm_inl     {σ1 σ2 : Ty} (t : ETerm σ1) : ETerm (ty.sum σ1 σ2)
     | eterm_inr     {σ1 σ2 : Ty} (t : ETerm σ2) : ETerm (ty.sum σ1 σ2)
+    | eterm_sext    {m n} (e : ETerm (ty.bvec m)) {p : IsTrue (m <=? n)} : ETerm (ty.bvec n)
+    | eterm_zext    {m n} (e : ETerm (ty.bvec m)) {p : IsTrue (m <=? n)} : ETerm (ty.bvec n)
     | eterm_tuple   {σs : Ctx Ty} (ts : Env ETerm σs) : ETerm (ty.tuple σs)
     | eterm_union   {U : unioni} (K : unionk U) (t : ETerm (unionk_ty U K)) : ETerm (ty.union U)
     | eterm_record  (R : recordi) (ts : NamedEnv ETerm (recordf_ty R)) : ETerm (ty.record R).
@@ -1487,6 +1491,8 @@ Module Type SymPropOn
         | term_not t => eterm_not (erase t)
         | term_inl t => eterm_inl (erase t)
         | term_inr t => eterm_inr (erase t)
+        | term_sext t => eterm_sext (erase t)
+        | term_zext t => eterm_zext (erase t)
         | term_tuple ts => eterm_tuple (env.map (fun _ => erase) ts)
         | term_union U K t => eterm_union K (erase t)
         | term_record R ts => eterm_record R (env.map (fun _ => erase) ts)
@@ -1568,6 +1574,10 @@ Module Type SymPropOn
             inl <$> inst_eterm t0
         | eterm_inr t0 =>
             inr <$> inst_eterm t0
+        | @eterm_sext _ _ t0 p =>
+            (fun v => bv.sext v) <$> inst_eterm t0
+        | @eterm_zext _ _ t0 p =>
+            (fun v => bv.zext v) <$> inst_eterm t0
         | @eterm_tuple σs ts =>
             envrec.of_env (σs := σs) <$> inst_env' ι inst_eterm ts
         | @eterm_union U K t0 =>
@@ -1663,6 +1673,8 @@ Module Type SymPropOn
         now rewrite EqDec.eq_dec_refl.
       - reflexivity.
       - now rewrite IHt1, IHt2.
+      - now rewrite IHt.
+      - now rewrite IHt.
       - now rewrite IHt.
       - now rewrite IHt.
       - now rewrite IHt.
