theories/Syntax/Expressions.v
@@ -28,6 +28,8 @@
 (******************************************************************************)
 
 From Coq Require Import
+     Arith.PeanoNat
+     Bool.Bool
      Strings.String
      ZArith.BinInt.
 From Katamaran Require Import
@@ -71,6 +73,8 @@ Module Type ExpressionsOn (Import TY : Types).
   | exp_not     (e : Exp Γ ty.bool) : Exp Γ ty.bool
   | exp_inl     {σ1 σ2 : Ty} : Exp Γ σ1 -> Exp Γ (ty.sum σ1 σ2)
   | exp_inr     {σ1 σ2 : Ty} : Exp Γ σ2 -> Exp Γ (ty.sum σ1 σ2)
+  | exp_sext    {m n} (e : Exp Γ (ty.bvec m)) {p : IsTrue (m <=? n)} : Exp Γ (ty.bvec n)
+  | exp_zext    {m n} (e : Exp Γ (ty.bvec m)) {p : IsTrue (m <=? n)} : Exp Γ (ty.bvec n)
   | exp_list    {σ : Ty} (es : list (Exp Γ σ)) : Exp Γ (ty.list σ)
   (* Experimental features *)
   | exp_bvec    {n} (es : Vector.t (Exp Γ ty.bool) n) : Exp Γ (ty.bvec n)
@@ -106,6 +110,8 @@ Module Type ExpressionsOn (Import TY : Types).
     Hypothesis (P_not     : forall e : Exp Γ ty.bool, P ty.bool e -> P ty.bool (exp_not e)).
     Hypothesis (P_inl     : forall (σ1 σ2 : Ty) (e : Exp Γ σ1), P σ1 e -> P (ty.sum σ1 σ2) (exp_inl e)).
     Hypothesis (P_inr     : forall (σ1 σ2 : Ty) (e : Exp Γ σ2), P σ2 e -> P (ty.sum σ1 σ2) (exp_inr e)).
+    Hypothesis (P_sext    : forall {m n} (p : IsTrue (Nat.leb m n)) (e : Exp Γ (ty.bvec m)), P (ty.bvec m) e -> P (ty.bvec n) (exp_sext e)).
+    Hypothesis (P_zext    : forall {m n} (p : IsTrue (Nat.leb m n)) (e : Exp Γ (ty.bvec m)), P (ty.bvec m) e -> P (ty.bvec n) (exp_zext e)).
     Hypothesis (P_list    : forall (σ : Ty) (es : list (Exp Γ σ)), PL es -> P (ty.list σ) (exp_list es)).
     Hypothesis (P_bvec    : forall (n : nat) (es : Vector.t (Exp Γ ty.bool) n), PV es -> P (ty.bvec n) (exp_bvec es)).
     Hypothesis (P_tuple   : forall (σs : Ctx Ty) (es : Env (Exp Γ) σs), PE es -> P (ty.tuple σs) (exp_tuple es)).
@@ -121,6 +127,8 @@ Module Type ExpressionsOn (Import TY : Types).
       | exp_not e                 => ltac:(apply P_not; auto)
       | exp_inl e                 => ltac:(apply P_inl; auto)
       | exp_inr e                 => ltac:(apply P_inr; auto)
+      | exp_sext e                => ltac:(apply P_sext; auto)
+      | exp_zext e                => ltac:(apply P_zext; auto)
       | exp_list es               => ltac:(apply P_list; induction es; cbn; auto using unit)
       | exp_bvec es               => ltac:(apply P_bvec; induction es; cbn; auto using unit)
       | exp_tuple es              => ltac:(apply P_tuple; induction es; cbn; auto using unit)
@@ -142,6 +150,8 @@ Module Type ExpressionsOn (Import TY : Types).
     | exp_not e           => negb (eval e δ)
     | exp_inl e           => inl (eval e δ)
     | exp_inr e           => inr (eval e δ)
+    | exp_sext e          => bv.sext (eval e δ)
+    | exp_zext e          => bv.zext (eval e δ)
     | exp_list es         => List.map (fun e => eval e δ) es
     | exp_bvec es         => Vector.t_rect
                                _ (fun m (_ : Vector.t (Exp Γ ty.bool) m) => bv m)
